n_mutualExAbs1_base.thy
@@ -1,0 +1,302 @@
+(*  Title:      HOL/Auth/n_mutualExAbs1_base.thy
+    Author:     Yongjian Li and Kaiqiang Duan, State Key Lab of Computer Science, Institute of Software, Chinese Academy of Sciences
+    Copyright    2016 State Key Lab of Computer Science, Institute of Software, Chinese Academy of Sciences
+*)
+
+header{*The n_mutualExAbs1 Protocol Case Study*} 
+
+theory n_mutualExAbs1_base imports paraTheory
+begin
+
+section{*Main definitions*}
+
+subsection{* Definitions of Constants*}
+definition I::"scalrValueType" where [simp]: "I\<equiv> enum ''control'' ''I''"
+definition T::"scalrValueType" where [simp]: "T\<equiv> enum ''control'' ''T''"
+definition C::"scalrValueType" where [simp]: "C\<equiv> enum ''control'' ''C''"
+definition E::"scalrValueType" where [simp]: "E\<equiv> enum ''control'' ''E''"
+definition true::"scalrValueType" where [simp]: "true\<equiv> boolV True"
+definition false::"scalrValueType" where [simp]: "false\<equiv> boolV False"
+
+
+
+subsection{*  Definitions of Parameterized Rules *}
+
+definition n_Try::"nat \<Rightarrow> rule" where [simp]:
+"n_Try  i\<equiv>
+let g = (eqn (IVar (Field (Para (Ident ''n'') i) ''st'')) (Const I)) in
+let s = (parallelList [(assign ((Field (Para (Ident ''n'') i) ''st''), (Const T)))]) in
+guard g s"
+
+definition n_Crit::"nat \<Rightarrow> rule" where [simp]:
+"n_Crit  i\<equiv>
+let g = (andForm (eqn (IVar (Field (Para (Ident ''n'') i) ''st'')) (Const T)) (eqn (IVar (Ident ''x'')) (Const true))) in
+let s = (parallelList [(assign ((Field (Para (Ident ''n'') i) ''st''), (Const C))), (assign ((Ident ''x''), (Const false))), (assign ((Field (Para (Ident ''n'') i) ''data''), (IVar (Ident ''memDATA''))))]) in
+guard g s"
+
+definition n_Exit::"nat \<Rightarrow> rule" where [simp]:
+"n_Exit  i\<equiv>
+let g = (eqn (IVar (Field (Para (Ident ''n'') i) ''st'')) (Const C)) in
+let s = (parallelList [(assign ((Field (Para (Ident ''n'') i) ''st''), (Const E)))]) in
+guard g s"
+
+definition n_Idle::"nat \<Rightarrow> rule" where [simp]:
+"n_Idle  i\<equiv>
+let g = (eqn (IVar (Field (Para (Ident ''n'') i) ''st'')) (Const E)) in
+let s = (parallelList [(assign ((Field (Para (Ident ''n'') i) ''st''), (Const I))), (assign ((Ident ''x''), (Const true))), (assign ((Ident ''memDATA''), (IVar (Field (Para (Ident ''n'') i) ''data''))))]) in
+guard g s"
+
+definition n_Store::"nat \<Rightarrow> nat \<Rightarrow> rule" where [simp]:
+"n_Store  i data\<equiv>
+let g = (eqn (IVar (Field (Para (Ident ''n'') i) ''st'')) (Const C)) in
+let s = (parallelList [(assign ((Field (Para (Ident ''n'') i) ''st''), (Const C))), (assign ((Ident ''x''), (Const false))), (assign ((Ident ''auxDATA''), (Const (index data)))), (assign ((Field (Para (Ident ''n'') i) ''data''), (Const (index data))))]) in
+guard g s"
+
+definition n_ABS_Store::"nat \<Rightarrow> nat \<Rightarrow> rule" where [simp]:
+"n_ABS_Store N data\<equiv>
+let g = (forallForm (down N) (\<lambda>j. (andForm (neg (eqn (IVar (Field (Para (Ident ''n'') j) ''st'')) (Const C))) (neg (eqn (IVar (Field (Para (Ident ''n'') j) ''st'')) (Const E)))))) in
+let s = (parallelList [(assign ((Ident ''x''), (Const false))), (assign ((Ident ''auxDATA''), (Const (index data))))]) in
+guard g s"
+
+definition n_ABS_Crit::"rule" where [simp]:
+"n_ABS_Crit  \<equiv>
+let g = (eqn (IVar (Ident ''x'')) (Const true)) in
+let s = (parallelList [(assign ((Ident ''x''), (Const false)))]) in
+guard g s"
+
+definition n_ABS_Idle::"nat \<Rightarrow> rule" where [simp]:
+"n_ABS_Idle N \<equiv>
+let g = (forallForm (down N) (\<lambda>j. (andForm (neg (eqn (IVar (Field (Para (Ident ''n'') j) ''st'')) (Const C))) (neg (eqn (IVar (Field (Para (Ident ''n'') j) ''st'')) (Const E)))))) in
+let s = (parallelList [(assign ((Ident ''x''), (Const true))), (assign ((Ident ''memDATA''), (IVar (Ident ''auxDATA''))))]) in
+guard g s"
+
+
+
+
+
+subsection{*The set of All actual Rules w.r.t. a Protocol Instance with Size $N$*}
+definition rules::"nat \<Rightarrow> rule set" where [simp]:
+"rules N \<equiv> {r.
+(\<exists> i. i\<le>N\<and>r=n_Try  i) \<or>
+(\<exists> i. i\<le>N\<and>r=n_Crit  i) \<or>
+(\<exists> i. i\<le>N\<and>r=n_Exit  i) \<or>
+(\<exists> i. i\<le>N\<and>r=n_Idle  i)
+}"
+
+definition  NC::"nat " where [simp]: "NC==1" 
+
+definition rulesAbs::"nat \<Rightarrow> rule set" where [simp]:
+"rulesAbs  N\<equiv> {r.
+(\<exists> i. i\<le>NC\<and>r=n_Crit  i) \<or>
+(\<exists> i. i\<le>NC\<and>r=n_Exit  i) \<or>
+(\<exists> i. i\<le>NC\<and>r=n_Idle  i) \<or>
+(\<exists> i data. i\<le>NC\<and>data\<le>N\<and>r=n_Store  i data) \<or>
+(\<exists> data. data\<le>N\<and>r=n_ABS_Store NC data) \<or>
+(r=n_ABS_Crit  ) \<or>
+(r=n_ABS_Idle NC )
+}"
+
+
+
+subsection{*Definitions of a Formally Parameterized Invariant Formulas*}
+
+
+
+subsection{*Definitions of  the Set of Invariant Formula Instances in a $N$-protocol Instance*}
+definition inv__1::"nat \<Rightarrow> nat \<Rightarrow> formula" where [simp]:
+"inv__1 p__Inv0 p__Inv1 \<equiv>
+(neg (andForm (eqn (IVar (Field (Para (Ident ''n'') p__Inv0) ''st'')) (Const C)) (eqn (IVar (Field (Para (Ident ''n'') p__Inv1) ''st'')) (Const C))))"
+
+definition inv__2::"nat \<Rightarrow> formula" where [simp]:
+"inv__2 p__Inv0 \<equiv>
+(neg (andForm (eqn (IVar (Field (Para (Ident ''n'') p__Inv0) ''st'')) (Const C)) (neg (eqn (IVar (Field (Para (Ident ''n'') p__Inv0) ''data'')) (IVar (Ident ''auxDATA''))))))"
+
+definition inv__3::"nat \<Rightarrow> formula" where [simp]:
+"inv__3 p__Inv0 \<equiv>
+(neg (andForm (eqn (IVar (Field (Para (Ident ''n'') p__Inv0) ''st'')) (Const E)) (neg (eqn (IVar (Field (Para (Ident ''n'') p__Inv0) ''data'')) (IVar (Ident ''auxDATA''))))))"
+
+definition inv__4::"nat \<Rightarrow> nat \<Rightarrow> formula" where [simp]:
+"inv__4 p__Inv0 p__Inv1 \<equiv>
+(neg (andForm (eqn (IVar (Field (Para (Ident ''n'') p__Inv0) ''st'')) (Const C)) (eqn (IVar (Field (Para (Ident ''n'') p__Inv1) ''st'')) (Const E))))"
+
+definition inv__5::"nat \<Rightarrow> nat \<Rightarrow> formula" where [simp]:
+"inv__5 p__Inv0 p__Inv1 \<equiv>
+(neg (andForm (eqn (IVar (Field (Para (Ident ''n'') p__Inv0) ''st'')) (Const E)) (eqn (IVar (Field (Para (Ident ''n'') p__Inv1) ''st'')) (Const E))))"
+
+definition inv__6::"nat \<Rightarrow> nat \<Rightarrow> formula" where [simp]:
+"inv__6 p__Inv0 p__Inv1 \<equiv>
+(neg (andForm (eqn (IVar (Field (Para (Ident ''n'') p__Inv0) ''st'')) (Const E)) (eqn (IVar (Field (Para (Ident ''n'') p__Inv1) ''st'')) (Const C))))"
+
+definition inv__7::"formula" where [simp]:
+"inv__7  \<equiv>
+(neg (andForm (eqn (IVar (Ident ''x'')) (Const true)) (neg (eqn (IVar (Ident ''memDATA'')) (IVar (Ident ''auxDATA''))))))"
+
+definition inv__8::"nat \<Rightarrow> formula" where [simp]:
+"inv__8 p__Inv0 \<equiv>
+(neg (andForm (eqn (IVar (Field (Para (Ident ''n'') p__Inv0) ''st'')) (Const C)) (eqn (IVar (Ident ''x'')) (Const true))))"
+
+definition inv__9::"nat \<Rightarrow> formula" where [simp]:
+"inv__9 p__Inv0 \<equiv>
+(neg (andForm (eqn (IVar (Field (Para (Ident ''n'') p__Inv0) ''st'')) (Const E)) (eqn (IVar (Ident ''x'')) (Const true))))"
+
+subsection{*Definitions of  the Set of Invariant Formula Instances in a $N$-protocol Instance*}
+definition invariants::"nat \<Rightarrow> formula set" where [simp]:
+"invariants N \<equiv> {f.
+(\<exists> p__Inv0 p__Inv1. p__Inv0\<le>N\<and>p__Inv1\<le>N\<and>p__Inv0~=p__Inv1\<and>f=inv__1  p__Inv0 p__Inv1) \<or>
+(\<exists> p__Inv0. p__Inv0\<le>N\<and>f=inv__2  p__Inv0) \<or>
+(\<exists> p__Inv0. p__Inv0\<le>N\<and>f=inv__3  p__Inv0) \<or>
+(\<exists> p__Inv0 p__Inv1. p__Inv0\<le>N\<and>p__Inv1\<le>N\<and>p__Inv0~=p__Inv1\<and>f=inv__4  p__Inv0 p__Inv1) \<or>
+(\<exists> p__Inv0 p__Inv1. p__Inv0\<le>N\<and>p__Inv1\<le>N\<and>p__Inv0~=p__Inv1\<and>f=inv__5  p__Inv0 p__Inv1) \<or>
+(\<exists> p__Inv0 p__Inv1. p__Inv0\<le>N\<and>p__Inv1\<le>N\<and>p__Inv0~=p__Inv1\<and>f=inv__6  p__Inv0 p__Inv1) \<or>
+(f=inv__7  ) \<or>
+(\<exists> p__Inv0. p__Inv0\<le>N\<and>f=inv__8  p__Inv0) \<or>
+(\<exists> p__Inv0. p__Inv0\<le>N\<and>f=inv__9  p__Inv0)
+}"
+
+definition invariantsAbs::" formula list" where [simp]:
+"invariantsAbs  \<equiv> [
+(inv__1  0 1) ,
+(inv__2  0),
+(inv__3 0),
+(inv__4  0 1),
+(inv__5  0 1),
+(inv__6  0 1) ,
+(inv__7  ) ,
+(inv__8  0) ,
+(inv__9  0)
+]"
+
+subsection{*Definitions of initial states*}
+
+definition initSpec0::"nat \<Rightarrow> formula" where [simp]:
+"initSpec0 N \<equiv> (forallForm (down N) (% i . (eqn (IVar (Field (Para (Ident ''n'') i) ''st'')) (Const I))))"
+
+definition initSpec1::"nat \<Rightarrow> formula" where [simp]:
+"initSpec1 N \<equiv> (forallForm (down N) (% i . (eqn (IVar (Field (Para (Ident ''n'') i) ''data'')) (Const (index 1)))))"
+
+definition initSpec2::"formula" where [simp]:
+"initSpec2  \<equiv> (eqn (IVar (Ident ''x'')) (Const true))"
+
+definition initSpec3::"formula" where [simp]:
+"initSpec3  \<equiv> (eqn (IVar (Ident ''auxDATA'')) (Const (index 1)))"
+
+definition initSpec4::"formula" where [simp]:
+"initSpec4  \<equiv> (eqn (IVar (Ident ''memDATA'')) (Const (index 1)))"
+
+definition allInitSpecs::"nat \<Rightarrow> formula list" where [simp]:
+"allInitSpecs N \<equiv> [
+(initSpec0 N),
+(initSpec1 N),
+(initSpec2 ),
+(initSpec3 ),
+(initSpec4 )
+]"
+
+definition allInitSpecsAbs::" formula list" where [simp]:
+"allInitSpecsAbs  \<equiv> [
+(initSpec0 NC), 
+(initSpec1 NC),
+(initSpec2  ),
+(initSpec3 ),
+(initSpec4 )
+]"
+
+axiomatization  where axiomOnf2 [simp,intro]:
+   "s \<in> reachableSet (set (allInitSpecs N )) (rules N) \<Longrightarrow>  1 < N \<Longrightarrow> 1 < i \<Longrightarrow> j<2 \<Longrightarrow>  formEval (f 0 1) s \<Longrightarrow> formEval (f i j) s"
+
+axiomatization  where axiomOnf1 [simp,intro]:
+   "s \<in> reachableSet (set (allInitSpecs N )) (rules N) \<Longrightarrow> 1 < N \<Longrightarrow> 1 < i \<Longrightarrow>formEval (f 0 ) s \<Longrightarrow> formEval (f i) s"
+
+lemma ruleSimId: 
+  assumes  a3:"\<forall>v. v\<in>varOfForm (pre r) \<longrightarrow> (\<exists>f. f \<in>F \<and>v \<in> varOfForm f)" and  
+  (*a5:"\<forall>f v va. v \<in> varOfForm f \<longrightarrow> f \<in>F \<longrightarrow>va\<in>varOfExp ( substExpByStatement (IVar v)  (act r))\<longrightarrow> (\<exists>f. f \<in> F \<and> va \<in> varOfForm f)" *)
+  a5:"\<forall>v a. a \<in> set (statement2Assigns (act r)) \<longrightarrow> v\<in>varOfExp ( substExpByStatement (IVar (fst a))  (act r))\<longrightarrow> (\<exists>f. f \<in> F \<and> v \<in> varOfForm f)"
+shows
+"trans_sim_on1 r r F"
+proof(unfold trans_sim_on1_def,(rule allI)+,(rule impI)+ ) 
+  fix s1 s2
+  assume b1:"formEval (pre r) s1 \<and> (\<forall> f. f \<in>F \<longrightarrow> formEval f s1 )" and b2:"state_sim_on1 s1 s2 F"
+  show "((state_sim_on1 (trans (act r) s1) (trans (act r) s2) F \<and> (formEval (pre r) s2 ))
+           \<or> state_sim_on1 (trans (act r) s1) s2 F)"
+  proof(rule disjI1,rule conjI)
+    show "state_sim_on1 (trans (act r) s1) (trans (act r) s2) F"
+    proof(unfold state_sim_on1_def,(rule allI)+,(rule impI)+)
+      fix f v
+      assume c1:"f \<in>F"  and c2:"v \<in>varOfForm f"
+      have c20:"expEval  (substExpByStatement (IVar v) (act r)) s1 = expEval (IVar v) (trans (act r) s1)" 
+        using preCondOnExp by blast
+     have c3:"expEval  (substExpByStatement (IVar v) (act r)) s2 = expEval (IVar v) (trans (act r) s2)"
+       using preCondOnExp by blast
+
+     have c4:"\<forall>v a. a \<in> set (statement2Assigns (act r)) \<longrightarrow> v\<in>varOfExp ( substExpByStatement (IVar (fst a))  (act r)) \<longrightarrow> s1(v) = s2 v"
+       using a5 b2 c1 c2 state_sim_on1_def by blast
+ 
+     have c5:"expEval (substExpByStatement (IVar v)  (act r)) s1 = expEval (substExpByStatement (IVar v)  (act r)) s2"
+     proof(case_tac "\<exists>a. a \<in> set (statement2Assigns (act r)) \<and> (fst a) =v")
+       assume d1:"\<exists>a. a \<in> set (statement2Assigns (act r)) \<and> (fst a) =v"
+       from d1 obtain as where d2:"as \<in> set (statement2Assigns (act r)) \<and> (fst as) =v" by blast
+         have d3:"\<forall>v.  v\<in>varOfExp ( substExpByStatement (IVar (fst as))  (act r)) \<longrightarrow> s1(v) = s2 v"
+           using c4 d2 by blast
+         then show "expEval (substExpByStatement (IVar v)  (act r)) s1 = expEval (substExpByStatement (IVar v)  (act r)) s2"
+           using agreeOnVarsOfExp d2 by blast
+       next
+         assume d1:"\<not>(\<exists>a. a \<in> set (statement2Assigns (act r)) \<and> (fst a) =v )"
+         have d1:"(substExpByStatement (IVar v)  (act r)) =   (IVar v)"  sorry
+         then show "expEval (substExpByStatement (IVar v)  (act r)) s1 = expEval (substExpByStatement (IVar v)  (act r)) s2"
+           using b2 c1 c2 by auto
+     qed     
+     show " trans (act r) s1 v =   trans (act r) s2 v"
+       using  c1 c2 c5 lemmaOnValOf by auto
+   qed
+ next
+   have "formEval (pre r) s1"
+     by (simp add: b1 )
+  have c4:"\<forall>va. va \<in> varOfForm  (pre r)\<longrightarrow> s1(va) = s2 va"
+    using  a3 b2 by auto 
+   show "formEval (pre r) s2"
+     using \<open>formEval (pre r) s1\<close> agreeOnVars c4 by blast 
+    
+ qed
+qed
+
+lemma setOfList[simp]: " {v. \<exists>f. f \<in> set flist \<and> v \<in> varOfForm f} = varOfFormList flist"
+proof(induct_tac flist,auto) qed
+
+lemma onF[simp,intro]: 
+  " varOfFormList invariantsAbs = 
+  { (Field (Para (Ident ''n'') 0) ''data''),varType.Field (Para (Ident ''n'') 0) ''st'' , varType.Field (Para (Ident ''n'') 1) ''st'',
+   (Ident ''x''),(Ident ''memDATA''),(Ident ''auxDATA'')  }"    
+(*{v. \<exists>f. f \<in> invariantsAbs \<and> v \<in> varOfForm f})*)
+  by auto
+ (* apply(simp)
+  apply(erule disjE)
+  apply(rule_tac x="inv__1 0 1" in exI,simp)
+  apply(erule disjE)
+  apply(rule_tac x="inv__1 0 1" in exI,simp)
+  apply(rule_tac x="inv__9 0 " in exI,simp)
+  done*)
+
+lemma lemmaOnTryLeNc:
+  assumes a1:"i\<le>NC" 
+  shows "trans_sim_on1 (n_Try  i) (n_Try  i) (set invariantsAbs)" (is "trans_sim_on1 ?r ?r ?F")
+proof(rule ruleSimId)
+  have "\<forall>v. v\<in>varOfForm (pre ?r) \<longrightarrow>  v \<in>(varOfFormList invariantsAbs)"
+    by(cut_tac a1, auto)
+  then show "\<forall>v. v\<in>varOfForm (pre ?r) \<longrightarrow>  v \<in>(varOfFormList invariantsAbs)"
+    sorry
+next
+  have  b1: "\<forall>v a. a \<in> set (statement2Assigns (act ?r)) \<longrightarrow> v\<in>varOfExp ( substExpByStatement (IVar (fst a))  (act ?r))\<longrightarrow>v \<in>varOfFormList invariantsAbs "
+   proof((rule allI)+,(rule impI)+,auto)
+  show "\<forall>v a. a \<in> set (statement2Assigns (act ?r)) \<longrightarrow> v\<in>varOfExp ( substExpByStatement (IVar (fst a))  (act ?r))\<longrightarrow> (\<exists>f. f \<in> ?F \<and> v \<in> varOfForm f)"
+  proof((rule allI)+,(rule impI)+)
+    fix v a
+    assume b1:"a \<in> set (statement2Assigns (act ?r)) " and b2:" v\<in>varOfExp ( substExpByStatement (IVar (fst a))  (act ?r))"
+    have "v=  (Para (Ident ''n'') i) \<or> v=(Ident ''x'')" by(cut_tac b1 b2,auto)
+    then have "v \<in> { (Para (Ident ''n'') 1) , (Para (Ident ''n'') 0), (Ident ''x'')}" 
+      apply (cut_tac a1, auto) done
+    then show "(\<exists>f. f \<in> ?F \<and> v \<in> varOfForm f)"
+      using onF by blast 
+      
+      apply(cut_tac a1,auto )
+    
+end
